src/tls/IV.fst
@@ -3,7 +3,8 @@ module IV
 open Mem
 open Pkg
 
-
+module M = LowStar.Modifies
+module DT = DefineTable
 
 /// A sample functionality for fresh, public initialization vectors,
 /// with the length of the byte vector as a basic agility
@@ -13,74 +14,69 @@ open Pkg
 /// There is no need for an idealization flag: the main (unconditional)
 /// property is that the vector is a function of the index; this
 /// vector is fresh whenever create is called instead of coerce.
+
 type idealRaw = b2t Flags.flag_Raw
+type len_of_id (ip:ipkg) = i:ip.t{model} -> keylen
 
 // SZ: [len_of_i] was implicit, but it can't be inferred from [i]. Made it explicit
-type rawlen (#ip:ipkg) (len_of_i:ip.t -> keylen) (i:ip.t) = len:keylen {len == len_of_i i}
-
-type raw (ip:ipkg) (len_of_i:ip.t -> keylen) (i:ip.t{ip.registered i}) = Bytes.lbytes32 (len_of_i i)
-
-noextract inline_for_extraction
-let shared_footprint_raw (ip:ipkg) (len_of_i:ip.t -> keylen): rset = Set.empty
+type rawlen (#ip:ipkg) (lid:len_of_id ip) (i:ip.t) = len:keylen {model ==> len == lid i}
+type raw (#ip:ipkg) (lid:len_of_id ip) (i:ip.t{ip.registered i}) = Bytes.bytes
+//  b:Bytes.bytes{model ==> Bytes.len b == lid i}
 
 noextract inline_for_extraction
-let footprint_raw (ip:ipkg) (len_of_i:ip.t -> keylen)
-  (#i:ip.t {ip.registered i}) (k:raw ip len_of_i i)
-  : GTot (s:rset{s `Set.disjoint` shared_footprint_raw ip len_of_i})
-  =
-  let fp = Set.empty in
-  let sfp = shared_footprint_raw ip len_of_i in
-  Set.lemma_equal_elim (fp `Set.intersect` sfp) Set.empty;
-  fp
-
-noextract inline_for_extraction
-let create_raw (ip:ipkg) (len_of_i:ip.t -> keylen)
-  (i:ip.t{ip.registered i}) (len:keylen {len = len_of_i i}):
-  ST (raw ip len_of_i i)
-  (requires fun h0 -> model)
-  (ensures fun h0 p h1 -> modifies_none h0 h1)
+let create_raw (#ip:ipkg) (lid:len_of_id ip)
+  (i:ip.t{ip.registered i}) (len:rawlen lid i):
+  ST (raw lid i)
+  (requires fun h0 -> model /\ lid i == len)
+  (ensures fun h0 p h1 -> M.modifies M.loc_none h0 h1 /\
+    fresh_loc M.loc_none h0 h1)
   = Random.sample32 len
 
-let coerceT_raw (ip:ipkg) (len_of_i:ip.t -> keylen)
+let coerceT_raw (#ip:ipkg) (lid:len_of_id ip)
   (i: ip.t {ip.registered i /\ (idealRaw ==> ~(ip.honest i))})
-  (len:keylen{len == len_of_i i}) (r: Bytes.lbytes32 len):
-  GTot (raw ip len_of_i i) = r
+  (len:rawlen lid i) (r:Bytes.lbytes32 len)
+  : GTot (raw lid i) 
+  = r
 
 inline_for_extraction
-let coerce_raw (ip: ipkg) (len_of_i: ip.t -> keylen)
+let coerce_raw (#ip: ipkg) (lid:len_of_id ip)
   (i: ip.t {ip.registered i /\ (idealRaw ==> ~(ip.honest i))})
-  (len:keylen {len == len_of_i i}) (r: Bytes.lbytes32 len):
-  ST (raw ip len_of_i i)
+  (len:rawlen lid i) (r: Bytes.lbytes32 len):
+  ST (raw lid i)
   (requires fun h0 -> True)
-  (ensures fun h0 k h1 -> k == coerceT_raw ip len_of_i i len r /\ modifies_none h0 h1)
+  (ensures fun h0 k h1 -> k == coerceT_raw lid i len r /\
+    M.modifies M.loc_none h0 h1)
   = r
 
 noextract
 inline_for_extraction
-let local_raw_pkg (ip:ipkg) (len_of_i:ip.t -> keylen) : local_pkg ip =
+let local_raw_pkg (#ip:ipkg) (lid:len_of_id ip)
+  : Pure (local_pkg ip)
+  (requires True) (ensures fun p -> LocalPkg?.key p == raw lid)
+  =
   LocalPkg
-    (raw ip len_of_i)
-    (rawlen #ip len_of_i)
-    (fun #i (n:rawlen len_of_i i) -> n)
+    (raw lid)
+    (rawlen lid)
+    (fun (i:ip.t{model}) -> lid i)
+    (fun #i (n:rawlen lid i) -> n)
     idealRaw
-    (shared_footprint_raw ip len_of_i)
-    (footprint_raw ip len_of_i)
+    (DT.empty_fp (raw lid))
     (fun #_ _ _ -> True) // no invariant
-    (fun _ _ _ _ _ -> ())
-    (fun #_ _ _ _ -> True) // no post-condition
-    (fun #_ _ _ _ _ _ -> ())
-    (create_raw ip len_of_i)
-    (coerceT_raw ip len_of_i)
-    (coerce_raw ip len_of_i)
+    (fun #_ _ _ _ _ -> ())
+    (create_raw lid)
+    (coerceT_raw lid)
+    (coerce_raw lid)
 
 noextract inline_for_extraction
-let rp (ip:ipkg) (len_of_i:ip.t -> keylen): ST (pkg ip)
+let rp (ip:ipkg) (lid:len_of_id ip): ST (pkg ip)
   (requires fun h0 -> True)
-  (ensures fun h0 p h1 -> modifies_one tls_define_region h0 h1 /\ p.package_invariant h1)
+  (ensures fun h0 p h1 ->
+    Pkg?.key p == raw lid /\
+    p == memoization (local_raw_pkg lid) p.define_table /\
+    p.package_invariant h1 /\
+    fresh_loc (DT.loc p.define_table) h0 h1)
   =
-  memoization_ST (local_raw_pkg ip len_of_i)
-
-// does this extract? 18-09-24 no
+  memoization_ST (local_raw_pkg lid)
 
 val discard: bool -> ST unit
   (requires (fun _ -> True))  (ensures (fun h0 _ h1 -> h0 == h1))
@@ -94,7 +90,7 @@ inline_for_extraction
 noextract
 private let ip : ipkg = Pkg.Idx id (fun _ -> True) (fun _ -> True) (fun _ -> true)
 
-private let len_of_i (i:id): keylen =
+private let len_of_i  (i:id): keylen =
   if i > 0 && i < 32 then UInt32.uint_to_t i
   else 32ul
 
@@ -108,13 +104,11 @@ let test() : ST unit
   print (Bytes.hex_of_bytes k);
 
   [@inline_let]
-  let p = local_raw_pkg ip len_of_i in
+  let p = local_raw_pkg #ip len_of_i in
   let v0 = LocalPkg?.coerce p 12 kl k in
   print (Bytes.hex_of_bytes v0);
-
-  let table = mem_alloc (fun n -> Bytes.lbytes n) in
-  [@inline_let]
-  let q = Pkg.memoization p table in
+  
+  let q = rp ip len_of_i in
   let v1 = Pkg?.coerce q 12 kl k in
   print (Bytes.hex_of_bytes v1);
   ()
